introduce map interface in lemmas + fix some proof

BoogieLang/Semantics.thy
@@ -233,8 +233,7 @@ lemma lookup_var_decl_global_3:
   by simp
 
 lemma lookup_vdecls_ty_global_4: "map_of (snd \<Lambda>) x = None \<Longrightarrow> lookup_vdecls_ty (fst \<Lambda>) x = Some t \<Longrightarrow> lookup_var_ty \<Lambda> x = Some t"
-  using lookup_var_decl_global  
-  by (fastforce simp: lookup_var_ty_def lookup_vdecls_ty_def)
+  using lookup_var_decl_global lookup_var_decl_ty_Some lookup_vdecls_ty_map_of by blast
 
 lemma lookup_vdecls_ty_global_5: "map_of (snd \<Lambda>) x = None \<Longrightarrow> lookup_var_ty \<Lambda> x = Some t \<Longrightarrow> lookup_vdecls_ty (fst \<Lambda>) x = Some t"
   using lookup_var_ty_def lookup_vdecls_ty_def
@@ -442,176 +441,176 @@ type_synonym 'struct_ty proc_context = "'struct_ty pdecl list"
 
 subsection \<open>Expression reduction (big-step semantics)\<close>
 
-inductive red_expr :: "'a absval_ty_fun \<Rightarrow> var_context \<Rightarrow> ('a, 'k) fun_interp \<Rightarrow> rtype_env \<Rightarrow> expr \<Rightarrow> ('a, 'k) nstate \<Rightarrow> ('a, 'k) val \<Rightarrow> bool"
-  ("_,_,_,_ \<turnstile> ((\<langle>_,_\<rangle>) \<Down> _)" [51,0,0,0,0,0] 81)
-  and red_exprs :: "'a absval_ty_fun \<Rightarrow> var_context \<Rightarrow> ('a, 'k) fun_interp \<Rightarrow> rtype_env \<Rightarrow> expr list \<Rightarrow> ('a, 'k) nstate \<Rightarrow> ('a, 'k) val list \<Rightarrow> bool"
-  ("_,_,_,_ \<turnstile> ((\<langle>_,_\<rangle>) [\<Down>] _)" [51,0,0,0,0,0] 81)
+inductive red_expr :: "'a absval_ty_fun \<Rightarrow> var_context \<Rightarrow> ('a, 'k) fun_interp \<Rightarrow> rtype_env \<Rightarrow> ('a, 'k) map_interface \<Rightarrow> expr \<Rightarrow> ('a, 'k) nstate \<Rightarrow> ('a, 'k) val \<Rightarrow> bool"
+  ("_,_,_,_,_ \<turnstile> ((\<langle>_,_\<rangle>) \<Down> _)" [51,0,0,0,0,0] 81)
+  and red_exprs :: "'a absval_ty_fun \<Rightarrow> var_context \<Rightarrow> ('a, 'k) fun_interp \<Rightarrow> rtype_env \<Rightarrow> ('a, 'k) map_interface \<Rightarrow> expr list \<Rightarrow> ('a, 'k) nstate \<Rightarrow> ('a, 'k) val list \<Rightarrow> bool"
+  ("_,_,_,_,_ \<turnstile> ((\<langle>_,_\<rangle>) [\<Down>] _)" [51,0,0,0,0,0] 81)
   for A :: "'a absval_ty_fun" and \<Lambda> :: "var_context" and \<Gamma> :: "('a, 'k) fun_interp"
   where 
-    RedVar: "\<lbrakk> lookup_var \<Lambda> n_s x = Some v \<rbrakk> \<Longrightarrow> A,\<Lambda>,\<Gamma>,\<Omega> \<turnstile> \<langle>(Var x), n_s\<rangle> \<Down> v"
-  | RedBVar: "\<lbrakk> binder_state n_s i = Some v \<rbrakk> \<Longrightarrow> A,\<Lambda>,\<Gamma>,\<Omega> \<turnstile> \<langle>BVar i, n_s\<rangle> \<Down> v"
-  | RedLit: "A,\<Lambda>,\<Gamma>,\<Omega> \<turnstile> \<langle>(Lit v), n_s\<rangle> \<Down> LitV v" 
-  | RedBinOp: "\<lbrakk>A,\<Lambda>,\<Gamma>,\<Omega> \<turnstile> \<langle>e1, n_s\<rangle> \<Down> v1; A,\<Lambda>,\<Gamma>,\<Omega> \<turnstile> \<langle>e2, n_s\<rangle> \<Down> v2;
+    RedVar: "\<lbrakk> lookup_var \<Lambda> n_s x = Some v \<rbrakk> \<Longrightarrow> A,\<Lambda>,\<Gamma>,\<Omega>,MI \<turnstile> \<langle>(Var x), n_s\<rangle> \<Down> v"
+  | RedBVar: "\<lbrakk> binder_state n_s i = Some v \<rbrakk> \<Longrightarrow> A,\<Lambda>,\<Gamma>,\<Omega>,MI \<turnstile> \<langle>BVar i, n_s\<rangle> \<Down> v"
+  | RedLit: "A,\<Lambda>,\<Gamma>,\<Omega>,MI \<turnstile> \<langle>(Lit v), n_s\<rangle> \<Down> LitV v" 
+  | RedBinOp: "\<lbrakk>A,\<Lambda>,\<Gamma>,\<Omega>,MI \<turnstile> \<langle>e1, n_s\<rangle> \<Down> v1; A,\<Lambda>,\<Gamma>,\<Omega>,MI \<turnstile> \<langle>e2, n_s\<rangle> \<Down> v2;
                  binop_eval_val bop v1 v2 = (Some v) \<rbrakk> \<Longrightarrow> 
-             A,\<Lambda>,\<Gamma>,\<Omega> \<turnstile> \<langle>(e1 \<guillemotleft>bop\<guillemotright> e2), n_s\<rangle> \<Down> v"
-  | RedUnOp: " \<lbrakk> A,\<Lambda>,\<Gamma>,\<Omega> \<turnstile> \<langle>e, n_s\<rangle> \<Down> v; unop_eval_val uop v = Some v' \<rbrakk> \<Longrightarrow> A,\<Lambda>,\<Gamma>,\<Omega> \<turnstile> \<langle>UnOp uop e, n_s\<rangle> \<Down> v'"
+             A,\<Lambda>,\<Gamma>,\<Omega>,MI \<turnstile> \<langle>(e1 \<guillemotleft>bop\<guillemotright> e2), n_s\<rangle> \<Down> v"
+  | RedUnOp: " \<lbrakk> A,\<Lambda>,\<Gamma>,\<Omega>,MI \<turnstile> \<langle>e, n_s\<rangle> \<Down> v; unop_eval_val uop v = Some v' \<rbrakk> \<Longrightarrow> A,\<Lambda>,\<Gamma>,\<Omega>,MI \<turnstile> \<langle>UnOp uop e, n_s\<rangle> \<Down> v'"
   | RedFunOp: "\<lbrakk> \<Gamma> f = Some f_interp;
-                A,\<Lambda>,\<Gamma>,\<Omega> \<turnstile> \<langle>args, n_s\<rangle> [\<Down>] v_args;
+                A,\<Lambda>,\<Gamma>,\<Omega>,MI \<turnstile> \<langle>args, n_s\<rangle> [\<Down>] v_args;
                 f_interp (map (instantiate \<Omega>) ty_args) v_args = Some v \<rbrakk> \<Longrightarrow>
-             A,\<Lambda>,\<Gamma>,\<Omega> \<turnstile> \<langle> FunExp f ty_args args, n_s \<rangle> \<Down> v"
-  | RedMapSelect: "\<lbrakk> A,\<Lambda>,\<Gamma>,\<Omega> \<turnstile> \<langle>e1, n_s\<rangle> \<Down> v1;
-                A,\<Lambda>,\<Gamma>,\<Omega> \<turnstile> \<langle>e2, n_s\<rangle> \<Down> v2;
-                select v1 v2 = Some v\<rbrakk> \<Longrightarrow>
-             A,\<Lambda>,\<Gamma>,\<Omega> \<turnstile> \<langle> MapSelect e1 e2, n_s \<rangle> \<Down> v"
+             A,\<Lambda>,\<Gamma>,\<Omega>,MI \<turnstile> \<langle> FunExp f ty_args args, n_s \<rangle> \<Down> v"
+  | RedMapSelect: "\<lbrakk> A,\<Lambda>,\<Gamma>,\<Omega>,MI \<turnstile> \<langle>e1, n_s\<rangle> \<Down> v1;
+                A,\<Lambda>,\<Gamma>,\<Omega>,MI \<turnstile> \<langle>e2, n_s\<rangle> \<Down> v2;
+                (map_select MI) v1 v2 = Some v\<rbrakk> \<Longrightarrow>
+             A,\<Lambda>,\<Gamma>,\<Omega>,MI \<turnstile> \<langle> MapSelect e1 e2, n_s \<rangle> \<Down> v"
   | RedCondExpTrue: 
-               "\<lbrakk> A,\<Lambda>,\<Gamma>,\<Omega> \<turnstile> \<langle>cond, n_s\<rangle> \<Down> (BoolV True); 
-                  A,\<Lambda>,\<Gamma>,\<Omega> \<turnstile> \<langle>thn, n_s\<rangle> \<Down> v \<rbrakk> \<Longrightarrow>
-            A,\<Lambda>,\<Gamma>,\<Omega> \<turnstile> \<langle> CondExp cond thn els, n_s \<rangle> \<Down> v"
+               "\<lbrakk> A,\<Lambda>,\<Gamma>,\<Omega>,MI \<turnstile> \<langle>cond, n_s\<rangle> \<Down> (BoolV True); 
+                  A,\<Lambda>,\<Gamma>,\<Omega>,MI \<turnstile> \<langle>thn, n_s\<rangle> \<Down> v \<rbrakk> \<Longrightarrow>
+            A,\<Lambda>,\<Gamma>,\<Omega>,MI \<turnstile> \<langle> CondExp cond thn els, n_s \<rangle> \<Down> v"
   | RedCondExpFalse: 
-               "\<lbrakk> A,\<Lambda>,\<Gamma>,\<Omega> \<turnstile> \<langle>cond, n_s\<rangle> \<Down> (BoolV False); 
-                  A,\<Lambda>,\<Gamma>,\<Omega> \<turnstile> \<langle>els, n_s\<rangle> \<Down> v \<rbrakk> \<Longrightarrow>
-            A,\<Lambda>,\<Gamma>,\<Omega> \<turnstile> \<langle> CondExp cond thn els, n_s \<rangle> \<Down> v"
-  | RedOld: "\<lbrakk> A,\<Lambda>,\<Gamma>,\<Omega> \<turnstile> \<langle> e, n_s\<lparr>global_state := old_global_state n_s \<rparr> \<rangle> \<Down> v\<rbrakk> \<Longrightarrow> 
-            A,\<Lambda>,\<Gamma>,\<Omega> \<turnstile> \<langle> Old e, n_s \<rangle> \<Down> v"
+               "\<lbrakk> A,\<Lambda>,\<Gamma>,\<Omega>,MI \<turnstile> \<langle>cond, n_s\<rangle> \<Down> (BoolV False); 
+                  A,\<Lambda>,\<Gamma>,\<Omega>,MI \<turnstile> \<langle>els, n_s\<rangle> \<Down> v \<rbrakk> \<Longrightarrow>
+            A,\<Lambda>,\<Gamma>,\<Omega>,MI \<turnstile> \<langle> CondExp cond thn els, n_s \<rangle> \<Down> v"
+  | RedOld: "\<lbrakk> A,\<Lambda>,\<Gamma>,\<Omega>,MI \<turnstile> \<langle> e, n_s\<lparr>global_state := old_global_state n_s \<rparr> \<rangle> \<Down> v\<rbrakk> \<Longrightarrow> 
+            A,\<Lambda>,\<Gamma>,\<Omega>,MI \<turnstile> \<langle> Old e, n_s \<rangle> \<Down> v"
   | RedExpListNil:
-    "A,\<Lambda>,\<Gamma>,\<Omega> \<turnstile> \<langle>[], n_s\<rangle> [\<Down>] []"
+    "A,\<Lambda>,\<Gamma>,\<Omega>,MI \<turnstile> \<langle>[], n_s\<rangle> [\<Down>] []"
   | RedExpListCons:
-    "\<lbrakk>A,\<Lambda>,\<Gamma>,\<Omega> \<turnstile> \<langle>e, n_s\<rangle> \<Down> v; A,\<Lambda>,\<Gamma>,\<Omega> \<turnstile> \<langle>es, n_s\<rangle> [\<Down>] vs \<rbrakk> \<Longrightarrow>
-      A,\<Lambda>,\<Gamma>,\<Omega> \<turnstile> \<langle>(e # es), n_s\<rangle> [\<Down>] (v # vs)"
+    "\<lbrakk>A,\<Lambda>,\<Gamma>,\<Omega>,MI \<turnstile> \<langle>e, n_s\<rangle> \<Down> v; A,\<Lambda>,\<Gamma>,\<Omega>,MI \<turnstile> \<langle>es, n_s\<rangle> [\<Down>] vs \<rbrakk> \<Longrightarrow>
+      A,\<Lambda>,\<Gamma>,\<Omega>,MI \<turnstile> \<langle>(e # es), n_s\<rangle> [\<Down>] (v # vs)"
 (* value quantification rules *)
   | RedForAllTrue:
-    "\<lbrakk>\<And>v. type_of_val A v = (instantiate \<Omega> ty) \<Longrightarrow> A,\<Lambda>,\<Gamma>,\<Omega> \<turnstile> \<langle>e, full_ext_env n_s v\<rangle> \<Down> LitV (LBool True) \<rbrakk> \<Longrightarrow> 
-     A,\<Lambda>,\<Gamma>,\<Omega> \<turnstile> \<langle>Forall ty e, n_s\<rangle> \<Down> LitV (LBool True)"
+    "\<lbrakk>\<And>v. type_of_val A v = (instantiate \<Omega> ty) \<Longrightarrow> A,\<Lambda>,\<Gamma>,\<Omega>,MI \<turnstile> \<langle>e, full_ext_env n_s v\<rangle> \<Down> LitV (LBool True) \<rbrakk> \<Longrightarrow> 
+     A,\<Lambda>,\<Gamma>,\<Omega>,MI \<turnstile> \<langle>Forall ty e, n_s\<rangle> \<Down> LitV (LBool True)"
   | RedForAllFalse:
-    "\<lbrakk>type_of_val A v = instantiate \<Omega> ty; A,\<Lambda>,\<Gamma>,\<Omega> \<turnstile> \<langle>e, full_ext_env n_s v\<rangle> \<Down> LitV (LBool False) \<rbrakk> \<Longrightarrow> 
-     A,\<Lambda>,\<Gamma>,\<Omega> \<turnstile> \<langle>Forall ty e, n_s\<rangle> \<Down> LitV (LBool False)"
+    "\<lbrakk>type_of_val A v = instantiate \<Omega> ty; A,\<Lambda>,\<Gamma>,\<Omega>,MI \<turnstile> \<langle>e, full_ext_env n_s v\<rangle> \<Down> LitV (LBool False) \<rbrakk> \<Longrightarrow> 
+     A,\<Lambda>,\<Gamma>,\<Omega>,MI \<turnstile> \<langle>Forall ty e, n_s\<rangle> \<Down> LitV (LBool False)"
   | RedExistsTrue:
-    "\<lbrakk>type_of_val A v = instantiate \<Omega> ty; A,\<Lambda>,\<Gamma>,\<Omega> \<turnstile> \<langle>e, full_ext_env n_s v\<rangle> \<Down> LitV (LBool True) \<rbrakk> \<Longrightarrow>
-     A,\<Lambda>,\<Gamma>,\<Omega> \<turnstile> \<langle>Exists ty e, n_s\<rangle> \<Down> LitV (LBool True)"
+    "\<lbrakk>type_of_val A v = instantiate \<Omega> ty; A,\<Lambda>,\<Gamma>,\<Omega>,MI \<turnstile> \<langle>e, full_ext_env n_s v\<rangle> \<Down> LitV (LBool True) \<rbrakk> \<Longrightarrow>
+     A,\<Lambda>,\<Gamma>,\<Omega>,MI \<turnstile> \<langle>Exists ty e, n_s\<rangle> \<Down> LitV (LBool True)"
   | RedExistsFalse:
-    "\<lbrakk>\<And>v. type_of_val A v = instantiate \<Omega> ty \<Longrightarrow> A,\<Lambda>,\<Gamma>,\<Omega> \<turnstile> \<langle>e, full_ext_env n_s v\<rangle> \<Down> LitV (LBool False) \<rbrakk> \<Longrightarrow>
-     A,\<Lambda>,\<Gamma>,\<Omega> \<turnstile> \<langle>Exists ty e, n_s\<rangle> \<Down> LitV (LBool False)"
+    "\<lbrakk>\<And>v. type_of_val A v = instantiate \<Omega> ty \<Longrightarrow> A,\<Lambda>,\<Gamma>,\<Omega>,MI \<turnstile> \<langle>e, full_ext_env n_s v\<rangle> \<Down> LitV (LBool False) \<rbrakk> \<Longrightarrow>
+     A,\<Lambda>,\<Gamma>,\<Omega>,MI \<turnstile> \<langle>Exists ty e, n_s\<rangle> \<Down> LitV (LBool False)"
 (* type quantification rules *)
   | RedForallT_True:
-    "\<lbrakk>\<And>\<tau>. closed \<tau> \<Longrightarrow> A,\<Lambda>,\<Gamma>,(\<tau>#\<Omega>) \<turnstile> \<langle>e, n_s\<rangle> \<Down> LitV (LBool True) \<rbrakk> \<Longrightarrow> 
-     A,\<Lambda>,\<Gamma>,\<Omega> \<turnstile> \<langle>ForallT e, n_s\<rangle> \<Down> LitV (LBool True)"
+    "\<lbrakk>\<And>\<tau>. closed \<tau> \<Longrightarrow> A,\<Lambda>,\<Gamma>,(\<tau>#\<Omega>),MI \<turnstile> \<langle>e, n_s\<rangle> \<Down> LitV (LBool True) \<rbrakk> \<Longrightarrow> 
+     A,\<Lambda>,\<Gamma>,\<Omega>,MI \<turnstile> \<langle>ForallT e, n_s\<rangle> \<Down> LitV (LBool True)"
   | RedForallT_False:
-    "\<lbrakk>closed \<tau>; A,\<Lambda>,\<Gamma>,(\<tau>#\<Omega>) \<turnstile> \<langle>e, n_s\<rangle> \<Down> LitV (LBool False) \<rbrakk> \<Longrightarrow>
-     A,\<Lambda>,\<Gamma>,\<Omega> \<turnstile> \<langle>ForallT e, n_s\<rangle> \<Down> LitV (LBool False)"
+    "\<lbrakk>closed \<tau>; A,\<Lambda>,\<Gamma>,(\<tau>#\<Omega>),MI \<turnstile> \<langle>e, n_s\<rangle> \<Down> LitV (LBool False) \<rbrakk> \<Longrightarrow>
+     A,\<Lambda>,\<Gamma>,\<Omega>,MI \<turnstile> \<langle>ForallT e, n_s\<rangle> \<Down> LitV (LBool False)"
   | RedExistsT_True:
-    "\<lbrakk>closed \<tau>; A,\<Lambda>,\<Gamma>,(\<tau>#\<Omega>) \<turnstile> \<langle>e, n_s\<rangle> \<Down> LitV (LBool True) \<rbrakk> \<Longrightarrow>
-     A,\<Lambda>,\<Gamma>,\<Omega> \<turnstile> \<langle>ExistsT e, n_s\<rangle> \<Down> LitV (LBool True)"
+    "\<lbrakk>closed \<tau>; A,\<Lambda>,\<Gamma>,(\<tau>#\<Omega>),MI \<turnstile> \<langle>e, n_s\<rangle> \<Down> LitV (LBool True) \<rbrakk> \<Longrightarrow>
+     A,\<Lambda>,\<Gamma>,\<Omega>,MI \<turnstile> \<langle>ExistsT e, n_s\<rangle> \<Down> LitV (LBool True)"
   | RedExistsT_False:
-    "\<lbrakk>\<And>\<tau>. closed \<tau> \<Longrightarrow> A,\<Lambda>,\<Gamma>,(\<tau>#\<Omega>) \<turnstile> \<langle>e, n_s\<rangle> \<Down> LitV (LBool False) \<rbrakk> \<Longrightarrow>
-     A,\<Lambda>,\<Gamma>,\<Omega> \<turnstile> \<langle>ExistsT e, n_s\<rangle> \<Down> LitV (LBool False)"
+    "\<lbrakk>\<And>\<tau>. closed \<tau> \<Longrightarrow> A,\<Lambda>,\<Gamma>,(\<tau>#\<Omega>),MI \<turnstile> \<langle>e, n_s\<rangle> \<Down> LitV (LBool False) \<rbrakk> \<Longrightarrow>
+     A,\<Lambda>,\<Gamma>,\<Omega>,MI \<turnstile> \<langle>ExistsT e, n_s\<rangle> \<Down> LitV (LBool False)"
 
-inductive_cases RedBinOp_case[elim!]: "A,\<Lambda>,\<Gamma>,\<Omega> \<turnstile> \<langle>(e1 \<guillemotleft>bop\<guillemotright> e2), n_s\<rangle> \<Down> v"
-inductive_cases RedUnOp_case[elim!]: "A,\<Lambda>,\<Gamma>,\<Omega> \<turnstile> \<langle>UnOp uop e1, n_s\<rangle> \<Down> v"
-inductive_cases RedFunOp_case[elim!]: "A,\<Lambda>,\<Gamma>,\<Omega> \<turnstile> \<langle> FunExp f ty_args args, n_s \<rangle> \<Down> v"
-inductive_cases RedCondExp_case[elim!]: "A,\<Lambda>,\<Gamma>,\<Omega> \<turnstile> \<langle> CondExp cond thn els, n_s \<rangle> \<Down> v"
-inductive_cases RedOld_case[elim!]: "A,\<Lambda>,\<Gamma>,\<Omega> \<turnstile> \<langle>Old  e, n_s\<rangle> \<Down> v"
-inductive_cases RedLit_case[elim!]: "A,\<Lambda>,\<Gamma>,\<Omega> \<turnstile> \<langle>(Lit l), n_s\<rangle> \<Down> LitV l"
-inductive_cases RedVar_case[elim!]: "A,\<Lambda>,\<Gamma>,\<Omega> \<turnstile> \<langle>(Var x), n_s\<rangle> \<Down> v"
-inductive_cases RedBVar_case[elim!]: "A,\<Lambda>,\<Gamma>,\<Omega> \<turnstile> \<langle>(BVar i), n_s\<rangle> \<Down> v"
-inductive_cases RedForallTrue_case: "A,\<Lambda>,\<Gamma>,\<Omega> \<turnstile> \<langle>Forall ty e, n_s\<rangle> \<Down> LitV (LBool True)"
-inductive_cases RedForallFalse_case: "A,\<Lambda>,\<Gamma>,\<Omega> \<turnstile> \<langle>Forall ty e, n_s\<rangle> \<Down> LitV (LBool False)"
+inductive_cases RedBinOp_case[elim!]: "A,\<Lambda>,\<Gamma>,\<Omega>,MI \<turnstile> \<langle>(e1 \<guillemotleft>bop\<guillemotright> e2), n_s\<rangle> \<Down> v"
+inductive_cases RedUnOp_case[elim!]: "A,\<Lambda>,\<Gamma>,\<Omega>,MI \<turnstile> \<langle>UnOp uop e1, n_s\<rangle> \<Down> v"
+inductive_cases RedFunOp_case[elim!]: "A,\<Lambda>,\<Gamma>,\<Omega>,MI \<turnstile> \<langle> FunExp f ty_args args, n_s \<rangle> \<Down> v"
+inductive_cases RedCondExp_case[elim!]: "A,\<Lambda>,\<Gamma>,\<Omega>,MI \<turnstile> \<langle> CondExp cond thn els, n_s \<rangle> \<Down> v"
+inductive_cases RedOld_case[elim!]: "A,\<Lambda>,\<Gamma>,\<Omega>,MI \<turnstile> \<langle>Old  e, n_s\<rangle> \<Down> v"
+inductive_cases RedLit_case[elim!]: "A,\<Lambda>,\<Gamma>,\<Omega>,MI \<turnstile> \<langle>(Lit l), n_s\<rangle> \<Down> LitV l"
+inductive_cases RedVar_case[elim!]: "A,\<Lambda>,\<Gamma>,\<Omega>,MI \<turnstile> \<langle>(Var x), n_s\<rangle> \<Down> v"
+inductive_cases RedBVar_case[elim!]: "A,\<Lambda>,\<Gamma>,\<Omega>,MI \<turnstile> \<langle>(BVar i), n_s\<rangle> \<Down> v"
+inductive_cases RedForallTrue_case: "A,\<Lambda>,\<Gamma>,\<Omega>,MI \<turnstile> \<langle>Forall ty e, n_s\<rangle> \<Down> LitV (LBool True)"
+inductive_cases RedForallFalse_case: "A,\<Lambda>,\<Gamma>,\<Omega>,MI \<turnstile> \<langle>Forall ty e, n_s\<rangle> \<Down> LitV (LBool False)"
 
 lemma red_cond_exp_cases:
-  assumes "A,\<Lambda>,\<Gamma>,\<Omega> \<turnstile> \<langle>CondExp cond thn els, n_s \<rangle> \<Down> v"
+  assumes "A,\<Lambda>,\<Gamma>,\<Omega>,MI \<turnstile> \<langle>CondExp cond thn els, n_s \<rangle> \<Down> v"
   obtains b
-  where "(A,\<Lambda>,\<Gamma>,\<Omega> \<turnstile> \<langle>cond, n_s\<rangle> \<Down> BoolV b) \<and> (A,\<Lambda>,\<Gamma>,\<Omega> \<turnstile> \<langle>if b then thn else els, n_s\<rangle> \<Down> v)"
+  where "(A,\<Lambda>,\<Gamma>,\<Omega>,MI \<turnstile> \<langle>cond, n_s\<rangle> \<Down> BoolV b) \<and> (A,\<Lambda>,\<Gamma>,\<Omega>,MI \<turnstile> \<langle>if b then thn else els, n_s\<rangle> \<Down> v)"
   using assms
   apply cases
    apply fastforce
   apply fastforce
   done
 
-definition expr_sat :: "'a absval_ty_fun \<Rightarrow> var_context \<Rightarrow> ('a, 'k) fun_interp \<Rightarrow> rtype_env \<Rightarrow> ('a, 'k) nstate \<Rightarrow> expr \<Rightarrow> bool"
-  where "expr_sat A \<Lambda> \<Gamma> \<Omega> n_s e = (A,\<Lambda>,\<Gamma>,\<Omega> \<turnstile> \<langle>e, n_s\<rangle> \<Down> LitV (LBool True))"
+definition expr_sat :: "'a absval_ty_fun \<Rightarrow> var_context \<Rightarrow> ('a, 'k) fun_interp \<Rightarrow> rtype_env \<Rightarrow> ('a, 'k) map_interface => ('a, 'k) nstate \<Rightarrow> expr \<Rightarrow> bool"
+  where "expr_sat A \<Lambda> \<Gamma> \<Omega> MI n_s e = (A,\<Lambda>,\<Gamma>,\<Omega>,MI \<turnstile> \<langle>e, n_s\<rangle> \<Down> LitV (LBool True))"
 
-definition expr_all_sat :: "'a absval_ty_fun \<Rightarrow> var_context \<Rightarrow> ('a, 'k) fun_interp \<Rightarrow> rtype_env \<Rightarrow> ('a, 'k) nstate \<Rightarrow> expr list \<Rightarrow> bool"
-  where "expr_all_sat A \<Lambda> \<Gamma> \<Omega> n_s es = list_all (expr_sat A \<Lambda> \<Gamma> \<Omega> n_s) es"
+definition expr_all_sat :: "'a absval_ty_fun \<Rightarrow> var_context \<Rightarrow> ('a, 'k) fun_interp \<Rightarrow> rtype_env \<Rightarrow> ('a, 'k) map_interface => ('a, 'k) nstate \<Rightarrow> expr list \<Rightarrow> bool"
+  where "expr_all_sat A \<Lambda> \<Gamma> \<Omega> MI n_s es = list_all (expr_sat A \<Lambda> \<Gamma> \<Omega> MI n_s) es"
 
-definition expr_exists_fail :: "'a absval_ty_fun \<Rightarrow> var_context \<Rightarrow> ('a, 'k) fun_interp \<Rightarrow> rtype_env \<Rightarrow> ('a, 'k) nstate \<Rightarrow> expr list \<Rightarrow> bool"
-  where "expr_exists_fail A \<Lambda> \<Gamma> \<Omega> n_s es = list_ex (expr_sat A \<Lambda> \<Gamma> \<Omega> n_s) es"
+definition expr_exists_fail :: "'a absval_ty_fun \<Rightarrow> var_context \<Rightarrow> ('a, 'k) fun_interp \<Rightarrow> rtype_env \<Rightarrow> ('a, 'k) map_interface => ('a, 'k) nstate \<Rightarrow> expr list \<Rightarrow> bool"
+  where "expr_exists_fail A \<Lambda> \<Gamma> \<Omega> MI n_s es = list_ex (expr_sat A \<Lambda> \<Gamma> \<Omega> MI n_s) es"
 
-definition where_clause_sat :: "'a absval_ty_fun \<Rightarrow> var_context \<Rightarrow> ('a, 'k) fun_interp \<Rightarrow> rtype_env \<Rightarrow> ('a, 'k) nstate \<Rightarrow> vdecl \<Rightarrow> bool"
-  where "where_clause_sat A \<Lambda> \<Gamma> \<Omega> n_s vd = (\<forall>x ty w. vd = (x,ty,Some w) \<longrightarrow> expr_sat A \<Lambda> \<Gamma> \<Omega> n_s w)"
+definition where_clause_sat :: "'a absval_ty_fun \<Rightarrow> var_context \<Rightarrow> ('a, 'k) fun_interp \<Rightarrow> rtype_env \<Rightarrow> ('a, 'k) map_interface => ('a, 'k) nstate \<Rightarrow> vdecl \<Rightarrow> bool"
+  where "where_clause_sat A \<Lambda> \<Gamma> \<Omega> MI n_s vd = (\<forall>x ty w. vd = (x,ty,Some w) \<longrightarrow> expr_sat A \<Lambda> \<Gamma> \<Omega> MI n_s w)"
 
-definition where_clauses_all_sat :: "'a absval_ty_fun \<Rightarrow> var_context \<Rightarrow> ('a, 'k) fun_interp \<Rightarrow> rtype_env \<Rightarrow> ('a, 'k) nstate \<Rightarrow> vdecls \<Rightarrow> bool"
-  where "where_clauses_all_sat A \<Lambda> \<Gamma> \<Omega> n_s vs = list_all (where_clause_sat A \<Lambda> \<Gamma> \<Omega> n_s) vs"
+definition where_clauses_all_sat :: "'a absval_ty_fun \<Rightarrow> var_context \<Rightarrow> ('a, 'k) fun_interp \<Rightarrow> rtype_env \<Rightarrow> ('a, 'k) map_interface => ('a, 'k) nstate \<Rightarrow> vdecls \<Rightarrow> bool"
+  where "where_clauses_all_sat A \<Lambda> \<Gamma> \<Omega> MI n_s vs = list_all (where_clause_sat A \<Lambda> \<Gamma> \<Omega> MI n_s) vs"
 
 (* where-clauses of global variables should be assumed without taking local variables into account, due to shadowing. *)
-definition where_clauses_all_sat_context :: "'a absval_ty_fun \<Rightarrow> var_context \<Rightarrow> ('a, 'k) fun_interp \<Rightarrow> rtype_env \<Rightarrow> ('a, 'k) nstate \<Rightarrow> bool"
-  where "where_clauses_all_sat_context A \<Lambda> \<Gamma> \<Omega> ns \<equiv> 
-           where_clauses_all_sat A (fst \<Lambda>, []) \<Gamma> \<Omega> ns (fst \<Lambda>) \<and> where_clauses_all_sat A \<Lambda> \<Gamma> \<Omega> ns (snd \<Lambda>)"
+definition where_clauses_all_sat_context :: "'a absval_ty_fun \<Rightarrow> var_context \<Rightarrow> ('a, 'k) fun_interp \<Rightarrow> rtype_env \<Rightarrow> ('a, 'k) map_interface => ('a, 'k) nstate \<Rightarrow> bool"
+  where "where_clauses_all_sat_context A \<Lambda> \<Gamma> \<Omega> MI ns \<equiv> 
+           where_clauses_all_sat A (fst \<Lambda>, []) \<Gamma> \<Omega> MI ns (fst \<Lambda>) \<and> where_clauses_all_sat A \<Lambda> \<Gamma> \<Omega> MI ns (snd \<Lambda>)"
 
 subsection \<open>Command reduction (big-step semantics)\<close>
 
-inductive red_cmd :: "'a absval_ty_fun \<Rightarrow> 'm proc_context \<Rightarrow> var_context \<Rightarrow> ('a, 'k) fun_interp \<Rightarrow> rtype_env \<Rightarrow> cmd \<Rightarrow> ('a, 'k) state \<Rightarrow> ('a, 'k) state \<Rightarrow> bool"
-  ("_,_,_,_,_ \<turnstile> ((\<langle>_,_\<rangle>) \<rightarrow>/ _)" [51,51,0,0,0] 81)
+inductive red_cmd :: "'a absval_ty_fun \<Rightarrow> 'm proc_context \<Rightarrow> var_context \<Rightarrow> ('a, 'k) fun_interp \<Rightarrow> rtype_env \<Rightarrow> ('a, 'k) map_interface \<Rightarrow> cmd \<Rightarrow> ('a, 'k) state \<Rightarrow> ('a, 'k) state \<Rightarrow> bool"
+  ("_,_,_,_,_,_ \<turnstile> ((\<langle>_,_\<rangle>) \<rightarrow>/ _)" [51,51,0,0,0] 81)
   for A :: "'a absval_ty_fun" and M :: "'m proc_context" and \<Lambda> :: var_context and  \<Gamma> :: "('a, 'k) fun_interp" and \<Omega> :: rtype_env
   where
-    RedAssertOk: "\<lbrakk> A,\<Lambda>,\<Gamma>,\<Omega> \<turnstile> \<langle>e, n_s\<rangle> \<Down> LitV (LBool True) \<rbrakk> \<Longrightarrow> 
-                 A,M,\<Lambda>,\<Gamma>,\<Omega> \<turnstile> \<langle>Assert e, Normal n_s\<rangle> \<rightarrow> Normal n_s"
-  | RedAssertFail: "\<lbrakk> A,\<Lambda>,\<Gamma>,\<Omega> \<turnstile> \<langle>e, n_s\<rangle> \<Down> LitV (LBool False) \<rbrakk> \<Longrightarrow> 
-                  A,M,\<Lambda>,\<Gamma>,\<Omega> \<turnstile> \<langle>Assert e, Normal n_s\<rangle> \<rightarrow> Failure"
-  | RedAssumeOk: "\<lbrakk> A,\<Lambda>,\<Gamma>,\<Omega> \<turnstile> \<langle>e, n_s\<rangle> \<Down> LitV (LBool True) \<rbrakk> \<Longrightarrow> 
-                A,M,\<Lambda>,\<Gamma>,\<Omega> \<turnstile> \<langle>Assume e, Normal n_s\<rangle> \<rightarrow> Normal n_s"
-  | RedAssumeMagic: "\<lbrakk> A,\<Lambda>,\<Gamma>,\<Omega> \<turnstile> \<langle>e, n_s\<rangle> \<Down> LitV (LBool False) \<rbrakk> \<Longrightarrow> 
-                A,M,\<Lambda>,\<Gamma>,\<Omega> \<turnstile> \<langle>Assume e, Normal n_s\<rangle> \<rightarrow> Magic"
+    RedAssertOk: "\<lbrakk> A,\<Lambda>,\<Gamma>,\<Omega>,MI \<turnstile> \<langle>e, n_s\<rangle> \<Down> LitV (LBool True) \<rbrakk> \<Longrightarrow> 
+                 A,M,\<Lambda>,\<Gamma>,\<Omega>,MI \<turnstile> \<langle>Assert e, Normal n_s\<rangle> \<rightarrow> Normal n_s"
+  | RedAssertFail: "\<lbrakk> A,\<Lambda>,\<Gamma>,\<Omega>,MI \<turnstile> \<langle>e, n_s\<rangle> \<Down> LitV (LBool False) \<rbrakk> \<Longrightarrow> 
+                  A,M,\<Lambda>,\<Gamma>,\<Omega>,MI \<turnstile> \<langle>Assert e, Normal n_s\<rangle> \<rightarrow> Failure"
+  | RedAssumeOk: "\<lbrakk> A,\<Lambda>,\<Gamma>,\<Omega>,MI \<turnstile> \<langle>e, n_s\<rangle> \<Down> LitV (LBool True) \<rbrakk> \<Longrightarrow> 
+                A,M,\<Lambda>,\<Gamma>,\<Omega>,MI \<turnstile> \<langle>Assume e, Normal n_s\<rangle> \<rightarrow> Normal n_s"
+  | RedAssumeMagic: "\<lbrakk> A,\<Lambda>,\<Gamma>,\<Omega>,MI \<turnstile> \<langle>e, n_s\<rangle> \<Down> LitV (LBool False) \<rbrakk> \<Longrightarrow> 
+                A,M,\<Lambda>,\<Gamma>,\<Omega>,MI \<turnstile> \<langle>Assume e, Normal n_s\<rangle> \<rightarrow> Magic"
   | RedAssign: "\<lbrakk> lookup_var_ty \<Lambda> x = Some ty; type_of_val A v = instantiate \<Omega> ty; 
-                  A,\<Lambda>,\<Gamma>,\<Omega> \<turnstile> \<langle>e, n_s\<rangle> \<Down> v \<rbrakk> \<Longrightarrow>
-               A,M,\<Lambda>,\<Gamma>,\<Omega> \<turnstile> \<langle>Assign x e, Normal n_s\<rangle> \<rightarrow>  Normal (update_var \<Lambda> n_s x v)"
+                  A,\<Lambda>,\<Gamma>,\<Omega>,MI \<turnstile> \<langle>e, n_s\<rangle> \<Down> v \<rbrakk> \<Longrightarrow>
+               A,M,\<Lambda>,\<Gamma>,\<Omega>,MI \<turnstile> \<langle>Assign x e, Normal n_s\<rangle> \<rightarrow>  Normal (update_var \<Lambda> n_s x v)"
   | RedHavocNormal: "\<lbrakk> lookup_var_decl \<Lambda> x = Some (ty,w); 
                  type_of_val A v = instantiate \<Omega> ty;
-                 \<And>cond. w = Some cond \<Longrightarrow> A,\<Lambda>,\<Gamma>,\<Omega> \<turnstile> \<langle>cond, (update_var \<Lambda> n_s x v)\<rangle> \<Down> BoolV True \<rbrakk> \<Longrightarrow>
-                 A,M,\<Lambda>,\<Gamma>,\<Omega> \<turnstile> \<langle>Havoc x, Normal n_s\<rangle> \<rightarrow> Normal (update_var \<Lambda> n_s x v)"
+                 \<And>cond. w = Some cond \<Longrightarrow> A,\<Lambda>,\<Gamma>,\<Omega>,MI \<turnstile> \<langle>cond, (update_var \<Lambda> n_s x v)\<rangle> \<Down> BoolV True \<rbrakk> \<Longrightarrow>
+                 A,M,\<Lambda>,\<Gamma>,\<Omega>,MI \<turnstile> \<langle>Havoc x, Normal n_s\<rangle> \<rightarrow> Normal (update_var \<Lambda> n_s x v)"
   | RedHavocMagic: "\<lbrakk> lookup_var_decl \<Lambda> x = Some (ty,Some(cond)); 
                  type_of_val A v = instantiate \<Omega> ty;
-                 A,\<Lambda>,\<Gamma>,\<Omega> \<turnstile> \<langle>cond, (update_var \<Lambda> n_s x v)\<rangle> \<Down> BoolV False \<rbrakk> \<Longrightarrow>
-                 A,M,\<Lambda>,\<Gamma>,\<Omega> \<turnstile> \<langle>Havoc x, Normal n_s\<rangle> \<rightarrow> Magic"
+                 A,\<Lambda>,\<Gamma>,\<Omega>,MI \<turnstile> \<langle>cond, (update_var \<Lambda> n_s x v)\<rangle> \<Down> BoolV False \<rbrakk> \<Longrightarrow>
+                 A,M,\<Lambda>,\<Gamma>,\<Omega>,MI \<turnstile> \<langle>Havoc x, Normal n_s\<rangle> \<rightarrow> Magic"
 (* TODO: where clauses for return variables *)
   | RedProcCallOkAndMagic: "\<lbrakk> map_of M m = Some msig; 
-      A,\<Lambda>,\<Gamma>,\<Omega> \<turnstile> \<langle>args, n_s\<rangle> [\<Down>] v_args;
+      A,\<Lambda>,\<Gamma>,\<Omega>,MI \<turnstile> \<langle>args, n_s\<rangle> [\<Down>] v_args;
       pre_ls = Map.empty( (map fst (proc_args msig )) [\<mapsto>] v_args  ) ;
-      expr_all_sat A (fst \<Lambda>, proc_args msig) \<Gamma> \<Omega> (n_s\<lparr>local_state := new_ls\<rparr>) (proc_checked_pres msig);
+      expr_all_sat A (fst \<Lambda>, proc_args msig) \<Gamma> \<Omega> MI (n_s\<lparr>local_state := new_ls\<rparr>) (proc_checked_pres msig);
       map (lookup_vdecls_ty (fst \<Lambda>)) (proc_modifs msig) = map Some ty_modifs;  
       map (type_of_val A) vs_modifs = map (instantiate \<Omega>) ty_modifs;
       map (type_of_val A) vs_ret = map (fst \<circ> snd) (proc_rets msig);      
       post_ls = pre_ls((map fst (proc_rets msig)) [\<mapsto>] vs_ret);
       post_gs = (global_state n_s)((proc_modifs msig) [\<mapsto>] vs_modifs);
       post_state = \<lparr>old_global_state = global_state n_s, global_state = post_gs, local_state = post_ls, binder_state = Map.empty\<rparr>;
-      post_success = expr_all_sat A (fst \<Lambda>, (proc_args msig)@(proc_rets msig)) \<Gamma> \<Omega> post_state (proc_all_posts msig);
-      post_fail = expr_exists_fail A (fst \<Lambda>, (proc_args msig)@(proc_rets msig)) \<Gamma> \<Omega> post_state (proc_all_posts msig);
+      post_success = expr_all_sat A (fst \<Lambda>, (proc_args msig)@(proc_rets msig)) \<Gamma> \<Omega> MI post_state (proc_all_posts msig);
+      post_fail = expr_exists_fail A (fst \<Lambda>, (proc_args msig)@(proc_rets msig)) \<Gamma> \<Omega> MI post_state (proc_all_posts msig);
       post_success \<or> post_fail;
       n_s' = n_s\<lparr>global_state := post_gs\<rparr>\<lparr>local_state := (local_state n_s)(rets [\<mapsto>] vs_ret)\<rparr> \<rbrakk> \<Longrightarrow>
-               A,M,\<Lambda>,\<Gamma>,\<Omega> \<turnstile> \<langle>ProcCall m args rets, Normal n_s\<rangle> \<rightarrow> (if post_success then Normal n_s' else Magic)"
+               A,M,\<Lambda>,\<Gamma>,\<Omega>,MI \<turnstile> \<langle>ProcCall m args rets, Normal n_s\<rangle> \<rightarrow> (if post_success then Normal n_s' else Magic)"
   | RedProcCallFail: "\<lbrakk> map_of M m = Some msig;
-      A,\<Lambda>,\<Gamma>,\<Omega> \<turnstile> \<langle>args, n_s\<rangle> [\<Down>] v_args;
+      A,\<Lambda>,\<Gamma>,\<Omega>,MI \<turnstile> \<langle>args, n_s\<rangle> [\<Down>] v_args;
       pre_ls = Map.empty( (map fst (proc_args msig )) [\<mapsto>] v_args  ) ;
-      expr_exists_fail A (fst \<Lambda>, proc_args msig) \<Gamma> \<Omega> (n_s\<lparr>local_state := new_ls\<rparr>) (proc_checked_pres msig) \<rbrakk> \<Longrightarrow>
-               A,M,\<Lambda>,\<Gamma>,\<Omega> \<turnstile> \<langle>ProcCall m args rets, Normal n_s\<rangle> \<rightarrow> Failure"
-  | RedPropagateMagic: "A,M,\<Lambda>,\<Gamma>,\<Omega> \<turnstile> \<langle>s, Magic\<rangle> \<rightarrow> Magic"
-  | RedPropagateFailure: "A,M,\<Lambda>,\<Gamma>,\<Omega> \<turnstile> \<langle>s, Failure\<rangle> \<rightarrow> Failure"
+      expr_exists_fail A (fst \<Lambda>, proc_args msig) \<Gamma> \<Omega> MI (n_s\<lparr>local_state := new_ls\<rparr>) (proc_checked_pres msig) \<rbrakk> \<Longrightarrow>
+               A,M,\<Lambda>,\<Gamma>,\<Omega>,MI \<turnstile> \<langle>ProcCall m args rets, Normal n_s\<rangle> \<rightarrow> Failure"
+  | RedPropagateMagic: "A,M,\<Lambda>,\<Gamma>,\<Omega>,MI \<turnstile> \<langle>s, Magic\<rangle> \<rightarrow> Magic"
+  | RedPropagateFailure: "A,M,\<Lambda>,\<Gamma>,\<Omega>,MI \<turnstile> \<langle>s, Failure\<rangle> \<rightarrow> Failure"
 
-inductive_cases RedAssertOk_case [elim]: "A,M,\<Lambda>,\<Gamma>,\<Omega> \<turnstile> \<langle>Assert e, Normal n_s\<rangle> \<rightarrow> Normal n_s"
-inductive_cases RedAssumeOk_case [elim]: "A,M,\<Lambda>,\<Gamma>,\<Omega> \<turnstile> \<langle>Assume e, Normal n_s\<rangle> \<rightarrow> Normal n_s"
-inductive_cases RedAssign_case: "A,M,\<Lambda>,\<Gamma>,\<Omega> \<turnstile> \<langle>Assign x e, Normal n_s\<rangle> \<rightarrow> Normal (update_var \<Lambda> n_s x v)"
-inductive_cases RedHavoc_case: "A,M,\<Lambda>,\<Gamma>,\<Omega> \<turnstile> \<langle>Havoc x, Normal n_s\<rangle> \<rightarrow> Normal (update_var \<Lambda> n_s x v)"
+inductive_cases RedAssertOk_case [elim]: "A,M,\<Lambda>,\<Gamma>,\<Omega>,MI \<turnstile> \<langle>Assert e, Normal n_s\<rangle> \<rightarrow> Normal n_s"
+inductive_cases RedAssumeOk_case [elim]: "A,M,\<Lambda>,\<Gamma>,\<Omega>,MI \<turnstile> \<langle>Assume e, Normal n_s\<rangle> \<rightarrow> Normal n_s"
+inductive_cases RedAssign_case: "A,M,\<Lambda>,\<Gamma>,\<Omega>,MI \<turnstile> \<langle>Assign x e, Normal n_s\<rangle> \<rightarrow> Normal (update_var \<Lambda> n_s x v)"
+inductive_cases RedHavoc_case: "A,M,\<Lambda>,\<Gamma>,\<Omega>,MI \<turnstile> \<langle>Havoc x, Normal n_s\<rangle> \<rightarrow> Normal (update_var \<Lambda> n_s x v)"
 
 text \<open>Command list reduction (big-step semantics)\<close>
 
-inductive red_cmd_list :: "'a absval_ty_fun \<Rightarrow> 'm proc_context \<Rightarrow> var_context \<Rightarrow> ('a, 'k) fun_interp \<Rightarrow> rtype_env \<Rightarrow> cmd list \<Rightarrow> ('a, 'k) state \<Rightarrow> ('a, 'k) state \<Rightarrow> bool"
-  ("_,_,_,_,_ \<turnstile> ((\<langle>_,_\<rangle>) [\<rightarrow>]/ _)" [51,0,0,0] 81)
+inductive red_cmd_list :: "'a absval_ty_fun \<Rightarrow> 'm proc_context \<Rightarrow> var_context \<Rightarrow> ('a, 'k) fun_interp \<Rightarrow> rtype_env \<Rightarrow> ('a, 'k) map_interface \<Rightarrow> cmd list \<Rightarrow> ('a, 'k) state \<Rightarrow> ('a, 'k) state \<Rightarrow> bool"
+  ("_,_,_,_,_,_ \<turnstile> ((\<langle>_,_\<rangle>) [\<rightarrow>]/ _)" [51,0,0,0] 81)
   for A :: "'a absval_ty_fun" and M :: "'m proc_context" and \<Lambda> :: var_context and \<Gamma> :: "('a, 'k) fun_interp" and \<Omega> :: rtype_env
   where
-    RedCmdListNil: "A,M,\<Lambda>,\<Gamma>,\<Omega> \<turnstile> \<langle>[],s\<rangle> [\<rightarrow>] s"
-  | RedCmdListCons: "\<lbrakk> A,M,\<Lambda>,\<Gamma>,\<Omega> \<turnstile> \<langle>c,s\<rangle> \<rightarrow> s''; A,M,\<Lambda>,\<Gamma>,\<Omega> \<turnstile> \<langle>cs,s''\<rangle> [\<rightarrow>] s' \<rbrakk> \<Longrightarrow> 
-                   A,M,\<Lambda>,\<Gamma>,\<Omega> \<turnstile> \<langle>(c # cs), s\<rangle> [\<rightarrow>] s'"
+    RedCmdListNil: "A,M,\<Lambda>,\<Gamma>,\<Omega>,MI \<turnstile> \<langle>[],s\<rangle> [\<rightarrow>] s"
+  | RedCmdListCons: "\<lbrakk> A,M,\<Lambda>,\<Gamma>,\<Omega>,MI \<turnstile> \<langle>c,s\<rangle> \<rightarrow> s''; A,M,\<Lambda>,\<Gamma>,\<Omega>,MI \<turnstile> \<langle>cs,s''\<rangle> [\<rightarrow>] s' \<rbrakk> \<Longrightarrow> 
+                   A,M,\<Lambda>,\<Gamma>,\<Omega>,MI \<turnstile> \<langle>(c # cs), s\<rangle> [\<rightarrow>] s'"
 
-inductive_cases RedCmdListNil_case [elim]: "A,M,\<Lambda>,\<Gamma>,\<Omega> \<turnstile> \<langle>[],s\<rangle> [\<rightarrow>] s"
-inductive_cases RedCmdListCons_case [elim]: "A,M,\<Lambda>,\<Gamma>,\<Omega> \<turnstile> \<langle>(c # cs), s\<rangle> [\<rightarrow>] s''"
+inductive_cases RedCmdListNil_case [elim]: "A,M,\<Lambda>,\<Gamma>,\<Omega>,MI \<turnstile> \<langle>[],s\<rangle> [\<rightarrow>] s"
+inductive_cases RedCmdListCons_case [elim]: "A,M,\<Lambda>,\<Gamma>,\<Omega>,MI \<turnstile> \<langle>(c # cs), s\<rangle> [\<rightarrow>] s''"
 
 subsection \<open>CFG reduction (small-step semantics)\<close>
 
@@ -621,13 +620,13 @@ inductive red_cfg :: "'a absval_ty_fun \<Rightarrow> mbodyCFG proc_context \<Rig
   ("_,_,_,_,_,_ \<turnstile> (_ -n\<rightarrow>/ _)" [51,0,0,0] 81)
   for A :: "'a absval_ty_fun" and M :: "mbodyCFG proc_context" and \<Lambda> :: var_context and \<Gamma> :: "('a, 'k) fun_interp" and \<Omega> :: rtype_env and G :: mbodyCFG
   where
-    RedNormalSucc: "\<lbrakk>node_to_block(G) ! n = cs; A,M,\<Lambda>,\<Gamma>,\<Omega> \<turnstile> \<langle>cs,Normal ns\<rangle> [\<rightarrow>] Normal ns'; List.member (out_edges(G) ! n) n'  \<rbrakk> \<Longrightarrow> 
+    RedNormalSucc: "\<lbrakk>node_to_block(G) ! n = cs; A,M,\<Lambda>,\<Gamma>,\<Omega>,MI \<turnstile> \<langle>cs,Normal ns\<rangle> [\<rightarrow>] Normal ns'; List.member (out_edges(G) ! n) n'  \<rbrakk> \<Longrightarrow> 
               A,M,\<Lambda>,\<Gamma>,\<Omega>,G  \<turnstile> (Inl n, Normal ns) -n\<rightarrow> (Inl n', Normal ns')"
-  | RedNormalReturn: "\<lbrakk>node_to_block(G)! n = cs; A,M,\<Lambda>,\<Gamma>,\<Omega> \<turnstile> \<langle>cs,Normal ns\<rangle> [\<rightarrow>] Normal ns'; (out_edges(G) ! n) = [] \<rbrakk> \<Longrightarrow> 
+  | RedNormalReturn: "\<lbrakk>node_to_block(G)! n = cs; A,M,\<Lambda>,\<Gamma>,\<Omega>,MI \<turnstile> \<langle>cs,Normal ns\<rangle> [\<rightarrow>] Normal ns'; (out_edges(G) ! n) = [] \<rbrakk> \<Longrightarrow> 
                A,M,\<Lambda>,\<Gamma>,\<Omega>,G  \<turnstile> (Inl n, Normal ns) -n\<rightarrow> (Inr (), Normal ns')"
-  | RedFailure: "\<lbrakk>node_to_block(G) ! n = cs; A,M,\<Lambda>,\<Gamma>,\<Omega> \<turnstile> \<langle>cs,Normal ns\<rangle> [\<rightarrow>] Failure \<rbrakk> \<Longrightarrow>
+  | RedFailure: "\<lbrakk>node_to_block(G) ! n = cs; A,M,\<Lambda>,\<Gamma>,\<Omega>,MI \<turnstile> \<langle>cs,Normal ns\<rangle> [\<rightarrow>] Failure \<rbrakk> \<Longrightarrow>
               A,M,\<Lambda>,\<Gamma>,\<Omega>,G  \<turnstile> (Inl n, Normal ns) -n\<rightarrow> (Inr (), Failure)"
-  | RedMagic: "\<lbrakk>node_to_block(G) ! n = cs; A,M,\<Lambda>,\<Gamma>,\<Omega> \<turnstile> \<langle>cs,Normal ns\<rangle> [\<rightarrow>] Magic \<rbrakk> \<Longrightarrow>
+  | RedMagic: "\<lbrakk>node_to_block(G) ! n = cs; A,M,\<Lambda>,\<Gamma>,\<Omega>,MI \<turnstile> \<langle>cs,Normal ns\<rangle> [\<rightarrow>] Magic \<rbrakk> \<Longrightarrow>
               A,M,\<Lambda>,\<Gamma>,\<Omega>,G  \<turnstile> (Inl n, Normal ns) -n\<rightarrow> (Inr (), Magic)"
 
 fun is_final_config :: "('a, 'k) cfg_config \<Rightarrow> bool"
@@ -706,23 +705,23 @@ qed
 subsection \<open>Procedure Correctness\<close>
 
 definition valid_configuration 
-  where "valid_configuration A \<Lambda> \<Gamma> \<Omega> posts m' s' \<equiv> 
+  where "valid_configuration A \<Lambda> \<Gamma> \<Omega> MI posts m' s' \<equiv> 
          s' \<noteq> Failure \<and> 
-         (is_final_config (m',s') \<longrightarrow> (\<forall>ns'. s' = Normal ns' \<longrightarrow> expr_all_sat A \<Lambda> \<Gamma> \<Omega> ns' posts))"
+         (is_final_config (m',s') \<longrightarrow> (\<forall>ns'. s' = Normal ns' \<longrightarrow> expr_all_sat A \<Lambda> \<Gamma> \<Omega> MI ns' posts))"
 
-definition proc_body_satisfies_spec :: "'a absval_ty_fun \<Rightarrow> mbodyCFG proc_context \<Rightarrow> var_context \<Rightarrow> ('a, 'k) fun_interp \<Rightarrow> rtype_env \<Rightarrow> expr list \<Rightarrow> expr list \<Rightarrow> mbodyCFG \<Rightarrow> ('a, 'k) nstate \<Rightarrow> bool"
-  where "proc_body_satisfies_spec A M \<Lambda> \<Gamma> \<Omega> pres posts mbody ns \<equiv>
-         expr_all_sat A \<Lambda> \<Gamma> \<Omega> ns pres \<longrightarrow> 
+definition proc_body_satisfies_spec :: "'a absval_ty_fun \<Rightarrow> mbodyCFG proc_context \<Rightarrow> var_context \<Rightarrow> ('a, 'k) fun_interp \<Rightarrow> rtype_env \<Rightarrow> ('a, 'k) map_interface \<Rightarrow> expr list \<Rightarrow> expr list \<Rightarrow> mbodyCFG \<Rightarrow> ('a, 'k) nstate \<Rightarrow> bool"
+  where "proc_body_satisfies_spec A M \<Lambda> \<Gamma> \<Omega> MI pres posts mbody ns \<equiv>
+         expr_all_sat A \<Lambda> \<Gamma> \<Omega> MI ns pres \<longrightarrow> 
           (\<forall> m' s'. (A, M, \<Lambda>, \<Gamma>, \<Omega>, mbody \<turnstile> (Inl (entry(mbody)), Normal ns) -n\<rightarrow>* (m',s')) \<longrightarrow> 
-                    valid_configuration A \<Lambda> \<Gamma> \<Omega> posts m' s')
+                    valid_configuration A \<Lambda> \<Gamma> \<Omega> MI posts m' s')
       "
 
 text \<open>\<^term>\<open>proc_body_satisfies_spec\<close> states when a procedure's CFG is correct w.r.t. postconditions \<^term>\<open>posts\<close> 
 under the assumption of preconditions \<^term>\<open>pres\<close>. To add support for where-clauses, one would need to 
 add an additional assumption here (proof generation does not support where-clauses currently).\<close>
 
-definition axioms_sat :: "'a absval_ty_fun \<Rightarrow> var_context \<Rightarrow> ('a, 'k) fun_interp \<Rightarrow> ('a, 'k) nstate \<Rightarrow> axiom list \<Rightarrow> bool"
-  where "axioms_sat A \<Lambda> \<Gamma> n_s as = list_all (expr_sat A \<Lambda> \<Gamma> [] n_s) as"
+definition axioms_sat :: "'a absval_ty_fun \<Rightarrow> var_context \<Rightarrow> ('a, 'k) fun_interp \<Rightarrow> ('a, 'k) map_interface \<Rightarrow> ('a, 'k) nstate \<Rightarrow> axiom list \<Rightarrow> bool"
+  where "axioms_sat A \<Lambda> \<Gamma> MI n_s as = list_all (expr_sat A \<Lambda> \<Gamma> [] MI n_s) as"
 
 definition state_restriction :: "('a, 'k) named_state \<Rightarrow> vdecls \<Rightarrow> ('a, 'k) named_state"
   where "state_restriction ns_orig vs x = 
@@ -732,8 +731,8 @@ definition nstate_global_restriction :: "('a, 'k) nstate \<Rightarrow> vdecls \<
   where "nstate_global_restriction ns vs = global_to_nstate (state_restriction (global_state ns) vs)"
 
 abbreviation axiom_assm
-  where "axiom_assm A \<Gamma> consts ns axioms \<equiv> 
-     (axioms_sat A (consts, []) \<Gamma> (nstate_global_restriction ns consts) axioms)"
+  where "axiom_assm A \<Gamma> MI consts ns axioms \<equiv> 
+     (axioms_sat A (consts, []) \<Gamma> MI (nstate_global_restriction ns consts) axioms)"
 
 text \<open>The following condition specifies what must hold for the list of constants with a unique modifier.
       The condition states that all corresponding values in the state must be distinct. Note that constants
@@ -747,23 +746,23 @@ text \<open>The following condition specifies what must hold for the list of con
 definition unique_constants_distinct :: "('a, 'k) named_state \<Rightarrow> vname list \<Rightarrow> bool"
   where "unique_constants_distinct ns xs \<longleftrightarrow> distinct (map (\<lambda>x. the (ns x)) xs)"
 
-fun proc_is_correct :: "'a absval_ty_fun \<Rightarrow> fdecls \<Rightarrow> vdecls \<Rightarrow> vname list \<Rightarrow> vdecls \<Rightarrow> axiom list \<Rightarrow> 'struct_ty2 procedure \<Rightarrow>
-                       ('a absval_ty_fun \<Rightarrow> 'struct_ty proc_context \<Rightarrow> var_context \<Rightarrow> ('a, 'k) fun_interp \<Rightarrow> rtype_env \<Rightarrow> expr list \<Rightarrow> expr list \<Rightarrow> 'struct_ty2 \<Rightarrow> ('a, 'k) nstate \<Rightarrow> bool) \<Rightarrow>
+fun proc_is_correct :: "'a absval_ty_fun \<Rightarrow> fdecls \<Rightarrow> vdecls \<Rightarrow> vname list \<Rightarrow> vdecls \<Rightarrow> axiom list \<Rightarrow> 'struct_ty2 procedure \<Rightarrow> ('a, 'k) map_interface \<Rightarrow>
+                       ('a absval_ty_fun \<Rightarrow> 'struct_ty proc_context \<Rightarrow> var_context \<Rightarrow> ('a, 'k) fun_interp \<Rightarrow> rtype_env \<Rightarrow> ('a, 'k) map_interface \<Rightarrow> expr list \<Rightarrow> expr list \<Rightarrow> 'struct_ty2 \<Rightarrow> ('a, 'k) nstate \<Rightarrow> bool) \<Rightarrow>
                          bool"
   where 
-    "proc_is_correct A fun_decls constants unique_consts global_vars axioms proc proc_body_satisfies_spec_general =  
+    "proc_is_correct A fun_decls constants unique_consts global_vars axioms proc MI proc_body_satisfies_spec_general =  
       (case proc_body(proc) of
         Some (locals, struct) \<Rightarrow> 
-          ( ( (\<forall>t. closed t \<longrightarrow> (\<exists>v. type_of_val A (v :: ('a, 'k) val) = t)) \<and> (\<forall>v. closed ((type_of_val A) v)) ) \<longrightarrow>
+          ( ( (\<forall>t. closed t \<longrightarrow> (\<exists>v. type_of_val A (v :: ('a, 'k) val) = t)) \<and> (\<forall>v. closed ((type_of_val A)  (v :: ('a, 'k) val))) ) \<longrightarrow>
           (\<forall> \<Gamma>. fun_interp_wf A fun_decls \<Gamma> \<longrightarrow>
           (
              (\<forall>\<Omega> gs ls. (list_all closed \<Omega> \<and> length \<Omega> = proc_ty_args proc) \<longrightarrow>        
              (state_typ_wf A \<Omega> gs (constants @ global_vars) \<longrightarrow>
               state_typ_wf A \<Omega> ls ((proc_args proc)@ (locals @ proc_rets proc)) \<longrightarrow>
               unique_constants_distinct gs unique_consts \<longrightarrow>
-              (axioms_sat A (constants, []) \<Gamma> (global_to_nstate (state_restriction gs constants)) axioms) \<longrightarrow>            
+              (axioms_sat A (constants, []) \<Gamma> MI (global_to_nstate (state_restriction gs constants)) axioms) \<longrightarrow>            
               (proc_body_satisfies_spec_general 
-                                        A [] (constants@global_vars, (proc_args proc)@(locals@(proc_rets proc))) \<Gamma> \<Omega> 
+                                        A [] (constants@global_vars, (proc_args proc)@(locals@(proc_rets proc))) \<Gamma> \<Omega> MI
                                        (proc_all_pres proc) (proc_checked_posts proc) struct
                                        \<lparr>old_global_state = gs, global_state = gs, local_state = ls, binder_state = Map.empty\<rparr> ) )
             )
@@ -791,7 +790,7 @@ fun proc_is_correct :: "'a absval_ty_fun \<Rightarrow> fdecls \<Rightarrow> vdec
       | None \<Rightarrow> True)"
 *)
 
-text \<open>\<^term>\<open>proc_is_correct A fun_decls constants unique_consts global_vars axioms proc proc_body_satisfies_spec_general\<close> gives the definition
+text \<open>\<^term>\<open>proc_is_correct A fun_decls constants unique_consts global_vars axioms proc MI proc_body_satisfies_spec_general\<close> gives the definition
 that a procedure \<^term>\<open>proc\<close> is correct w.r.t. the type interpretation \<^term>\<open>A\<close> the function declarations \<open>fun_decls\<close>, 
 constants \<^term>\<open>constants\<close>, global variables \<^term>\<open>global_vars\<close> and Boogie axioms \<^term>\<open>axioms\<close>. 
 \<^term>\<open>unique_consts\<close> denotes the list of constants with a unique modifier.
@@ -800,7 +799,7 @@ Since the current proof generation does not support procedure calls yet, we just
 procedure context to the empty list here. 
 
 In our certificates, we prove 
-\<^prop>\<open>\<And>A. proc_is_correct A fun_decls constants unique_consts global_vars axioms proc proc_body_satisfies_spec_general\<close>.
+\<^prop>\<open>\<And>A. proc_is_correct A fun_decls constants unique_consts global_vars axioms proc MI proc_body_satisfies_spec_general\<close>.
 That is, we prove procedure correctness for every type interpretation (\<And> is a universal quantifier at 
 the meta level). Note that for certain type interpretations procedure correctness is trivial (see
 the definition of \<^const>\<open>proc_is_correct\<close>).
@@ -811,71 +810,71 @@ subsection \<open>Properties of the semantics\<close>
 text \<open>Expression evaluation is deterministic\<close>
 
 lemma expr_eval_determ: 
-shows "((A,\<Lambda>,\<Gamma>,\<Omega> \<turnstile> \<langle>e1, s\<rangle> \<Down> v) \<Longrightarrow> ((A,\<Lambda>,\<Gamma>,\<Omega> \<turnstile> \<langle>e1, s\<rangle> \<Down> v') \<Longrightarrow> v = v'))"  
-    and "(A,\<Lambda>,\<Gamma>,\<Omega> \<turnstile> \<langle>es, s\<rangle> [\<Down>] vs) \<Longrightarrow> (A,\<Lambda>,\<Gamma>,\<Omega> \<turnstile> \<langle>es, s\<rangle> [\<Down>] vs') \<Longrightarrow> vs = vs' "
+shows "((A,\<Lambda>,\<Gamma>,\<Omega>,MI \<turnstile> \<langle>e1, s\<rangle> \<Down> v) \<Longrightarrow> ((A,\<Lambda>,\<Gamma>,\<Omega>,MI \<turnstile> \<langle>e1, s\<rangle> \<Down> v') \<Longrightarrow> v = v'))"  
+    and "(A,\<Lambda>,\<Gamma>,\<Omega>,MI \<turnstile> \<langle>es, s\<rangle> [\<Down>] vs) \<Longrightarrow> (A,\<Lambda>,\<Gamma>,\<Omega>,MI \<turnstile> \<langle>es, s\<rangle> [\<Down>] vs') \<Longrightarrow> vs = vs' "
 proof (induction arbitrary: v' and vs' rule: red_expr_red_exprs.inducts)
-  case (RedVar n_s x v \<Omega>)
-  assume "A,\<Lambda>,\<Gamma>,\<Omega> \<turnstile> \<langle>Var x,n_s\<rangle> \<Down> v'"
+  case (RedVar n_s x v \<Omega> MI)
+  assume "A,\<Lambda>,\<Gamma>,\<Omega>,MI \<turnstile> \<langle>Var x,n_s\<rangle> \<Down> v'"
   then show ?case using \<open>lookup_var \<Lambda> n_s x = Some v\<close> by (cases; simp)
 next
-  case (RedBVar n_s i v \<Omega>)
+  case (RedBVar n_s i v \<Omega> MI)
   assume "binder_state n_s i = Some v"
-  assume "A,\<Lambda>,\<Gamma>,\<Omega> \<turnstile> \<langle>BVar i,n_s\<rangle> \<Down> v'"
+  assume "A,\<Lambda>,\<Gamma>,\<Omega>,MI \<turnstile> \<langle>BVar i,n_s\<rangle> \<Down> v'"
   then show ?case using \<open>binder_state n_s i = Some v\<close> by (cases; simp)
 next
-  case (RedLit \<Omega> l n_s)
-  assume "A,\<Lambda>,\<Gamma>,\<Omega> \<turnstile> \<langle>Lit l,n_s\<rangle> \<Down> v'"
+  case (RedLit \<Omega> MI l n_s)
+  assume "A,\<Lambda>,\<Gamma>,\<Omega>,MI \<turnstile> \<langle>Lit l,n_s\<rangle> \<Down> v'"
   then show ?case by (cases; simp)
 next
-  case (RedBinOp \<Omega> e1 n_s v1 e2 v2 bop v)
+  case (RedBinOp \<Omega> MI e1 n_s v1 e2 v2 bop v)
   from RedBinOp.prems show ?case
   proof (cases)
     fix v1' v2'
-    assume "A,\<Lambda>,\<Gamma>,\<Omega> \<turnstile> \<langle>e1,n_s\<rangle> \<Down> v1'" hence "v1 = v1'" using RedBinOp.IH by simp
-    assume "A,\<Lambda>,\<Gamma>,\<Omega> \<turnstile> \<langle>e2,n_s\<rangle> \<Down> v2'" hence "v2 = v2'" using RedBinOp.IH by simp
+    assume "A,\<Lambda>,\<Gamma>,\<Omega>,MI \<turnstile> \<langle>e1,n_s\<rangle> \<Down> v1'" hence "v1 = v1'" using RedBinOp.IH by simp
+    assume "A,\<Lambda>,\<Gamma>,\<Omega>,MI \<turnstile> \<langle>e2,n_s\<rangle> \<Down> v2'" hence "v2 = v2'" using RedBinOp.IH by simp
     assume "binop_eval_val bop v1' v2' = Some v'"
     with \<open>v1 = v1'\<close> \<open>v2 = v2'\<close> show ?thesis using RedBinOp.hyps by simp
   qed
 next
-  case (RedUnOp \<Omega> e n_s v uop v' veval)
+  case (RedUnOp \<Omega> MI e n_s v uop v' veval)
   from RedUnOp.prems show ?case
   proof (cases)
     fix v2
-    assume "A,\<Lambda>,\<Gamma>,\<Omega> \<turnstile> \<langle>e,n_s\<rangle> \<Down> v2" hence "v2 = v" using RedUnOp.IH by simp
+    assume "A,\<Lambda>,\<Gamma>,\<Omega>,MI \<turnstile> \<langle>e,n_s\<rangle> \<Down> v2" hence "v2 = v" using RedUnOp.IH by simp
     assume "unop_eval_val uop v2 = Some veval"
     with \<open>v2 = v\<close> show ?thesis using RedUnOp.hyps by simp
   qed
 next
-  case (RedFunOp f f_interp \<Omega> args n_s v_args ty_args v v')
+  case (RedFunOp f f_interp \<Omega> MI args n_s v_args ty_args v v')
   from RedFunOp.prems show ?case
   proof (cases)
     fix v_args' f_interp'
-    assume "A,\<Lambda>,\<Gamma>,\<Omega> \<turnstile> \<langle>args,n_s\<rangle> [\<Down>] v_args'" hence "v_args = v_args'" using RedFunOp.IH by simp
+    assume "A,\<Lambda>,\<Gamma>,\<Omega>,MI \<turnstile> \<langle>args,n_s\<rangle> [\<Down>] v_args'" hence "v_args = v_args'" using RedFunOp.IH by simp
     assume "\<Gamma> f = Some f_interp'" hence "f_interp = f_interp'" using RedFunOp.IH by simp
     assume "f_interp' (map (instantiate \<Omega>) ty_args) v_args' = Some v'"
     thus ?case using \<open>v_args = v_args'\<close> \<open>f_interp = f_interp'\<close> using RedFunOp.hyps by simp
   qed
 next
-  case (RedMapSelect \<Omega> e1 n_s v1 e2 v2 v)
+  case (RedMapSelect \<Omega> MI e1 n_s v1 e2 v2 v)
   from RedMapSelect.prems show ?case
   proof (cases)
     fix v1' v2'
-    assume "A,\<Lambda>,\<Gamma>,\<Omega> \<turnstile> \<langle>e1,n_s\<rangle> \<Down> v1'" hence "v1 = v1'" using RedMapSelect.IH by simp
-    assume "A,\<Lambda>,\<Gamma>,\<Omega> \<turnstile> \<langle>e2,n_s\<rangle> \<Down> v2'" hence "v2 = v2'" using RedMapSelect.IH by simp
-    assume "select v1' v2' = Some v'"
+    assume "A,\<Lambda>,\<Gamma>,\<Omega>,MI \<turnstile> \<langle>e1,n_s\<rangle> \<Down> v1'" hence "v1 = v1'" using RedMapSelect.IH by simp
+    assume "A,\<Lambda>,\<Gamma>,\<Omega>,MI \<turnstile> \<langle>e2,n_s\<rangle> \<Down> v2'" hence "v2 = v2'" using RedMapSelect.IH by simp
+    assume "(map_select MI) v1' v2' = Some v'"
     with \<open>v1 = v1'\<close> \<open>v2 = v2'\<close> show ?thesis using RedMapSelect.hyps by simp
   qed
 next
   case (RedExpListNil n_s vs')
   thus ?case by (cases; simp)
 next
-  case (RedExpListCons \<Omega> e n_s v es vs' vs'')
-  assume "A,\<Lambda>,\<Gamma>,\<Omega> \<turnstile> \<langle>e # es,n_s\<rangle> [\<Down>] vs''"
+  case (RedExpListCons \<Omega> MI e n_s v es vs' vs'')
+  assume "A,\<Lambda>,\<Gamma>,\<Omega>,MI \<turnstile> \<langle>e # es,n_s\<rangle> [\<Down>] vs''"
   thus ?case 
   proof cases
     fix w ws      
-    assume "A,\<Lambda>,\<Gamma>,\<Omega> \<turnstile> \<langle>e,n_s\<rangle> \<Down> w" hence "v = w" using RedExpListCons.IH by simp
-    assume "A,\<Lambda>,\<Gamma>,\<Omega> \<turnstile> \<langle>es,n_s\<rangle> [\<Down>] ws" hence "ws = vs'" using RedExpListCons.IH by simp  
+    assume "A,\<Lambda>,\<Gamma>,\<Omega>,MI \<turnstile> \<langle>e,n_s\<rangle> \<Down> w" hence "v = w" using RedExpListCons.IH by simp
+    assume "A,\<Lambda>,\<Gamma>,\<Omega>,MI \<turnstile> \<langle>es,n_s\<rangle> [\<Down>] ws" hence "ws = vs'" using RedExpListCons.IH by simp  
     moreover assume "vs'' = w # ws"
     ultimately show ?thesis using \<open>v = w\<close>  by simp
   qed
@@ -918,11 +917,11 @@ next
   thus ?case by (blast elim: red_expr.cases)    
 qed
 
-lemma red_exprs_length: "A,\<Lambda>,\<Gamma>,\<Omega> \<turnstile> \<langle>es, n_s\<rangle> [\<Down>] vs \<Longrightarrow> length es = length vs"
+lemma red_exprs_length: "A,\<Lambda>,\<Gamma>,\<Omega>,MI \<turnstile> \<langle>es, n_s\<rangle> [\<Down>] vs \<Longrightarrow> length es = length vs"
   by (induction vs arbitrary: es; erule red_exprs.cases; simp)
    
 lemma step_nil_same:
-  assumes A1: "A,M,\<Lambda>,\<Gamma>,\<Omega> \<turnstile> \<langle>[], s\<rangle> [\<rightarrow>] s''"
+  assumes A1: "A,M,\<Lambda>,\<Gamma>,\<Omega>,MI \<turnstile> \<langle>[], s\<rangle> [\<rightarrow>] s''"
   shows "s = s''"
 proof -
   from A1 show ?thesis by (cases; auto)
@@ -937,13 +936,13 @@ lemma no_out_edges_return:
   by (simp add: red_cfg.simps member_rec(2)) 
 
 lemma magic_stays_cmd:
-  assumes "A,M,\<Lambda>,\<Gamma>,\<Omega> \<turnstile> \<langle>c, Magic\<rangle> \<rightarrow> s'"
+  assumes "A,M,\<Lambda>,\<Gamma>,\<Omega>,MI \<turnstile> \<langle>c, Magic\<rangle> \<rightarrow> s'"
   shows "s' = Magic"
   using assms
   by (cases rule: red_cmd.cases)
 
 lemma magic_stays_cmd_list_aux:
-  assumes "A,M,\<Lambda>,\<Gamma>,\<Omega> \<turnstile> \<langle>cs, s\<rangle> [\<rightarrow>] s'" and "s = Magic"
+  assumes "A,M,\<Lambda>,\<Gamma>,\<Omega>,MI \<turnstile> \<langle>cs, s\<rangle> [\<rightarrow>] s'" and "s = Magic"
   shows   "s' = Magic"
   using assms
 proof (induct rule: red_cmd_list.induct)
@@ -955,22 +954,22 @@ next
 qed
 
 lemma magic_stays_cmd_list:
-  assumes "A,M,\<Lambda>,\<Gamma>,\<Omega> \<turnstile> \<langle>cs, Magic\<rangle> [\<rightarrow>] s'"
+  assumes "A,M,\<Lambda>,\<Gamma>,\<Omega>,MI \<turnstile> \<langle>cs, Magic\<rangle> [\<rightarrow>] s'"
   shows "s' = Magic"
   using assms
   by (simp add: magic_stays_cmd_list_aux)
 
-lemma magic_red_cmd_list: "A,M,\<Lambda>',\<Gamma>,\<Omega> \<turnstile> \<langle>cs,Magic\<rangle> [\<rightarrow>] Magic"
+lemma magic_red_cmd_list: "A,M,\<Lambda>',\<Gamma>,\<Omega>,MI \<turnstile> \<langle>cs,Magic\<rangle> [\<rightarrow>] Magic"
   by (induction cs) (auto intro: red_cmd_list.intros RedPropagateMagic)
 
 lemma failure_stays_cmd:
-  assumes "A,M,\<Lambda>,\<Gamma>,\<Omega> \<turnstile> \<langle>c, Failure\<rangle> \<rightarrow> s'"
+  assumes "A,M,\<Lambda>,\<Gamma>,\<Omega>,MI \<turnstile> \<langle>c, Failure\<rangle> \<rightarrow> s'"
   shows "s' = Failure"
   using assms
   by (cases rule: red_cmd.cases)
 
 lemma failure_stays_cmd_list_aux:
-  assumes "A,M,\<Lambda>,\<Gamma>,\<Omega> \<turnstile> \<langle>cs, s\<rangle> [\<rightarrow>] s'" and "s = Failure"
+  assumes "A,M,\<Lambda>,\<Gamma>,\<Omega>,MI \<turnstile> \<langle>cs, s\<rangle> [\<rightarrow>] s'" and "s = Failure"
   shows   "s' = Failure"
   using assms
 proof (induct rule: red_cmd_list.induct)
@@ -982,12 +981,12 @@ next
 qed
 
 lemma failure_stays_cmd_list:
-  assumes "A,M,\<Lambda>,\<Gamma>,\<Omega> \<turnstile> \<langle>cs, Failure\<rangle> [\<rightarrow>] s'"
+  assumes "A,M,\<Lambda>,\<Gamma>,\<Omega>,MI \<turnstile> \<langle>cs, Failure\<rangle> [\<rightarrow>] s'"
   shows "s' = Failure"
   using assms
   by (simp add: failure_stays_cmd_list_aux)
 
-lemma failure_red_cmd_list: "A,M,\<Lambda>',\<Gamma>,\<Omega> \<turnstile> \<langle>cs,Failure\<rangle> [\<rightarrow>] Failure"
+lemma failure_red_cmd_list: "A,M,\<Lambda>',\<Gamma>,\<Omega>,MI \<turnstile> \<langle>cs,Failure\<rangle> [\<rightarrow>] Failure"
   by (induction cs) (auto intro: red_cmd_list.intros RedPropagateFailure)
 
 lemma finished_remains: 
@@ -1004,8 +1003,8 @@ next
 qed
 
 lemma forall_red:
-  assumes "A,\<Lambda>,\<Gamma>,\<Omega> \<turnstile> \<langle>Forall ty e, n_s\<rangle> \<Down> v"
-  shows "\<exists>b. (v = LitV (LBool b)) \<and> (b = (\<forall>v'. type_of_val A v' = (instantiate \<Omega> ty) \<longrightarrow> A, \<Lambda>, \<Gamma>, \<Omega> \<turnstile> \<langle>e, full_ext_env n_s v'\<rangle> \<Down> LitV (LBool True)))"
+  assumes "A,\<Lambda>,\<Gamma>,\<Omega>,MI \<turnstile> \<langle>Forall ty e, n_s\<rangle> \<Down> v"
+  shows "\<exists>b. (v = LitV (LBool b)) \<and> (b = (\<forall>v'. type_of_val A v' = (instantiate \<Omega> ty) \<longrightarrow> A, \<Lambda>, \<Gamma>, \<Omega>, MI \<turnstile> \<langle>e, full_ext_env n_s v'\<rangle> \<Down> LitV (LBool True)))"
   using assms
 proof (cases)
   case RedForAllTrue
@@ -1017,8 +1016,8 @@ next
 qed
 
 lemma exists_red:
-  assumes "A, \<Lambda>, \<Gamma>, \<Omega> \<turnstile> \<langle>Exists ty e, n_s\<rangle> \<Down> v"
-  shows "\<exists>b. (v = LitV (LBool b)) \<and> (b = (\<exists>v'. (type_of_val A v' = (instantiate \<Omega> ty)) \<and> A,\<Lambda>,\<Gamma>,\<Omega> \<turnstile> \<langle>e, full_ext_env n_s v'\<rangle> \<Down> LitV (LBool True)))"
+  assumes "A, \<Lambda>, \<Gamma>, \<Omega>, MI \<turnstile> \<langle>Exists ty e, n_s\<rangle> \<Down> v"
+  shows "\<exists>b. (v = LitV (LBool b)) \<and> (b = (\<exists>v'. (type_of_val A v' = (instantiate \<Omega> ty)) \<and> A,\<Lambda>,\<Gamma>,\<Omega>,MI \<turnstile> \<langle>e, full_ext_env n_s v'\<rangle> \<Down> LitV (LBool True)))"
   using assms
 proof (cases)
   case RedExistsTrue
@@ -1031,14 +1030,14 @@ qed
 
 (* TODO: make more precise *)
 lemma forallt_red_bool:
-  assumes "A, \<Lambda>, \<Gamma>, \<Omega> \<turnstile> \<langle>ForallT e, n_s\<rangle> \<Down> v"
+  assumes "A, \<Lambda>, \<Gamma>, \<Omega>, MI \<turnstile> \<langle>ForallT e, n_s\<rangle> \<Down> v"
   shows "\<exists>b. (v = LitV (LBool b))"
   using assms
   by (cases; auto)
 
 (* TODO: make more precise *)
 lemma existst_red_bool:
-  assumes "A, \<Lambda>, \<Gamma>, \<Omega> \<turnstile> \<langle>ExistsT e, n_s\<rangle> \<Down> v"
+  assumes "A, \<Lambda>, \<Gamma>, \<Omega>, MI \<turnstile> \<langle>ExistsT e, n_s\<rangle> \<Down> v"
   shows "\<exists>b. (v = LitV (LBool b))"
   using assms
   by (cases; auto)
